write_header

src/QUIC.Impl.Header.Parse.fst
@@ -8,6 +8,9 @@ friend QUIC.Spec.Header.Parse
 module LP = LowParse.Low.Base
 module Public = QUIC.Impl.Header.Public
 module U8 = FStar.UInt8
+module SecretBuffer = QUIC.Secret.Buffer
+module Spec = QUIC.Spec.Header.Parse
+module PN = QUIC.Impl.PacketNumber
 
 [@"opaque_to_smt"]
 let impl_short_protected_bits
@@ -48,8 +51,6 @@ let public_header_len_correct
   (public_header_len h == Public.header_len (p_header h))
 = ()
 
-module Spec = QUIC.Spec.Header.Parse
-
 #push-options "--z3rlimit 1024 --query_stats"
 
 let public_g_header_p_header
@@ -64,6 +65,22 @@ let public_g_header_p_header
     Public.g_header (p_header h) m == ph
   )
 = ()
+
+let public_header_len_correct'
+  (h: header)
+  (m: HS.mem)
+  (pn: PN.packet_number_t)
+: Lemma (
+    let gh = g_header h m pn in
+    let cid_len = dcid_len h in
+    let last = last_packet_number gh in
+    let (| ph, pn' |) = synth_header_recip cid_len last gh in
+    Public.g_header (p_header h) m == ph /\
+    U32.v (public_header_len h) == Seq.length (LP.serialize (Public.serialize_header cid_len) ph) 
+  )
+= public_header_len_correct h;
+  public_g_header_p_header h m pn;
+  Public.header_len_correct (dcid_len h) m (p_header h)
 
 #restart-solver
 
@@ -81,6 +98,7 @@ let header_len_correct
   serialize_header_eq cid_len last gh;
   Public.header_len_correct cid_len m (p_header h);
   public_header_len_correct h;
+  public_header_len_correct' h m pn;
   assert (Seq.length (LP.serialize (Public.serialize_header cid_len) ph) == U32.v (public_header_len h));
   if is_retry h
   then
@@ -91,4 +109,56 @@ let header_len_correct
     assert (Secret.v (header_len h) == Spec.header_len (g_header h m pn))
   end
 
+let last_pn
+  (is_retry: bool)
+  (pn: PN.packet_number_t)
+: Tot PN.last_packet_number_t
+= if is_retry
+  then Secret.to_u64 0uL
+  else
+    let cond = Secret.lognot_one_bit (pn `Secret.secrets_are_equal_62` Secret.to_u64 0uL) in
+    pn `Secret.sub` cond
+
+let last_pn_correct
+  (h: header)
+  (m: HS.mem)
+  (pn: PN.packet_number_t)
+: Lemma
+  (last_packet_number (g_header h m pn) == last_pn (is_retry h) pn)
+= ()
+
+let write_header
+  h pn out out_len
+= let m = HST.get () in
+  public_header_len_correct' h m pn;
+  let cid_len = dcid_len h in
+  let last = last_pn (is_retry h) pn in
+  last_pn_correct h m pn;
+  let ph = p_header h in
+  serialize_header_eq cid_len last (g_header h m pn);
+  let len = Public.write_header cid_len ph out out_len in
+  if is_retry h
+  then ()
+  else begin
+    assert (len == Public.header_len ph);
+    let pn_len = pn_length h in
+    let m1 = HST.get () in
+    SecretBuffer.with_buffer_hide
+      #unit
+      out
+      len
+      (len `U32.add` 4ul)
+      m1
+      B.loc_none
+      B.loc_none
+      0ul 0ul 0ul 4ul 0ul 0ul
+      (fun _ contl cont _ _ ->
+        contl == LP.serialize (Public.serialize_header cid_len) (Public.g_header ph m) /\
+        Seq.slice cont 0 (Secret.v pn_len) `Seq.equal` LP.serialize (PN.serialize_packet_number last pn_len) pn
+      )
+      (fun _ _ bs _ ->
+        PN.write_packet_number last pn_len pn bs
+      )
+  end
+  
 #pop-options
