src/QUIC.Impl.Header.Parse.fsti
@@ -8,6 +8,9 @@ module Seq = FStar.Seq
 module PN = QUIC.Spec.PacketNumber.Base
 module Secret = QUIC.Secret.Int
 module Spec = QUIC.Spec.Header.Parse
+module U8 = FStar.UInt8
+module B = LowStar.Buffer
+module HST = FStar.HyperStack.ST
 
 val header_len_correct
   (h: header)
@@ -15,3 +18,24 @@ val header_len_correct
   (pn: PN.packet_number_t)
 : Lemma
   (Secret.v (header_len h) == Spec.header_len (g_header h m pn))
+
+val write_header
+  (h: header)
+  (pn: PN.packet_number_t)
+  (out: B.buffer U8.t)
+  (out_len: U32.t { U32.v out_len <= B.length out })
+: HST.Stack unit
+  (requires (fun h0 ->
+    header_live h h0 /\
+    B.live h0 out /\
+    B.loc_disjoint (header_footprint h) (B.loc_buffer out) /\
+    U32.v (public_header_len h) + 4 <= U32.v out_len // needs more space than just pn_length to write pn in constant time
+  ))
+  (ensures (fun h0 _ h1 ->
+    let gh = g_header h h0 pn in
+    let s = format_header gh in
+    let len = header_len h in
+    B.modifies (B.loc_buffer out) h0 h1 /\
+    Secret.v len <= U32.v out_len /\
+    Seq.slice (B.as_seq h1 out) 0 (Secret.v len) `Seq.equal` s 
+  ))
